src/ndep/SymEval.v
@@ -1,36 +1,10 @@
 Require Import List Bedrock.DepList Word Memory.
 Require Import Heaps SepTheoryX.
-Require Import Bedrock.ndep.Expr Bedrock.ndep.SepExpr Bedrock.ndep.Provers.
+Require Import Bedrock.ndep.Expr Bedrock.ndep.SepExpr.
+Require Import Bedrock.ndep.Env.
 
 Set Implicit Arguments.
 Set Strict Implicit.
-
-Section UpdatePosition.
-  Variable T : Type.
-
-  Fixpoint updatePosition (n : nat) (v : T) (ls : list T) : list T :=
-    match n , ls with
-      | 0 , nil => v :: nil
-      | 0 , _ :: b => v :: b 
-      | S n , nil => v :: updatePosition n v nil
-      | S n , a :: b => a :: updatePosition n v b
-    end.
-
-  Lemma updatePosition_eq : forall n types' t,
-    nth_error (updatePosition n t types') n = Some t.
-  Proof.
-    induction n; simpl; destruct types'; eauto.
-  Defined.
-
-  Lemma updatePosition_neq : forall t n types' m,
-    n <> m ->
-    nth_error types' n <> None ->
-    nth_error (updatePosition m t types') n = nth_error types' n.
-  Proof.
-    clear.
-    induction n; destruct types'; destruct m; simpl; intros; try solve [ exfalso; auto; omega ]; auto.
-  Defined.
-End UpdatePosition.
 
 (** * These are generic search functions *)
 Section search_read_write.
@@ -527,7 +501,7 @@ Module EvaluatorPlugin (B : Heap) (ST : SepTheoryX.SepTheoryXType B) : Evaluator
 
 End EvaluatorPlugin.
 
-
+(*
 Module BedrockEvaluator (B : Heap) (ST : SepTheoryX.SepTheoryXType B).
   Module Import SEP := SepExpr B ST.
   Require Import IL.
@@ -536,9 +510,27 @@ Module BedrockEvaluator (B : Heap) (ST : SepTheoryX.SepTheoryXType B).
   Require Import Bedrock.SepTac.
 
   Variable types' : list type.
-  Definition types := bedrock_types ++ types'.
-  Definition pcT := tvType 0.
-  Definition stT := tvType 1.
+  Definition wIdx := 0.
+  Definition stIdx := 1.
+  Print bedrock_types.
+  Definition W_type := 
+    {| Impl := W
+     ; Expr.Eq := fun x y : W =>
+       match weq x y with
+         | left pf => Some pf
+         | right _ => None
+       end |}.
+  Definition state_type := 
+    SEP.defaultType (settings * state)%type.
+
+  Definition wT := tvType wIdx.
+  Definition stT := tvType stIdx.
+
+  Definition deltaT := ((wIdx, W_type) :: (stIdx, state_type) :: nil).
+
+  Definition types := repr deltaT types'.
+
+  Definition castor := cast_repr_tvar deltaT.
 
   (** These the reflected version of the IL, it essentially 
    ** replaces all uses of W with expr types so that the value
@@ -589,12 +581,11 @@ Module BedrockEvaluator (B : Heap) (ST : SepTheoryX.SepTheoryXType B).
 
   (** Symbolic State **)
   Record SymState : Type :=
-  { SymMem  : SEP.SHeap types pcT stT
+  { SymMem  : SEP.SHeap types wT stT
   ; SymRegs : SymRegType
   }.
 
   (** This has to be connected to the type of the intermediate representation **)
-  Definition tvWord := tvType 0.
 
   Definition sym_evalRval (rv : sym_rvalue) (ss : SymState) : option (expr types) :=
     match rv with
@@ -665,19 +656,32 @@ Module BedrockEvaluator (B : Heap) (ST : SepTheoryX.SepTheoryXType B).
     end.
 *)
 
-  Variable sfuncs : SEP.sfunctions types pcT stT.
+  Variable sfuncs : SEP.sfunctions types wT stT.
 
   (* Denotation functions *)
   Section sym_denote.
     Variable uvars vars : env types.
 
+    Print cast_repr.
+
+    Definition exprD_repr (e : expr types) (t : nat) : option (match nth_error_repr deltaT types' t with
+                                                                 | None => Empty_set
+                                                                 | Some t => Impl t
+                                                               end) :=
+      let d := exprD funcs uvars vars e (tvType t) in
+      @cast_repr _ (fun t => 
+        option match t with
+                 | None => Empty_set
+                 | Some t => Impl t 
+               end) deltaT types' t d.
+
     Definition sym_regsD (rs : SymRegType) : option regs :=
       match rs with
         | (sp, rp, rv) =>
           match 
-            exprD funcs uvars vars sp tvWord ,
-            exprD funcs uvars vars rp tvWord ,
-            exprD funcs uvars vars rv tvWord 
+            exprD_repr sp wIdx ,
+            exprD_repr rp wIdx ,
+            exprD_repr rv wIdx
             with
             | Some sp , Some rp , Some rv =>
                 Some (fun r => 
@@ -694,12 +698,12 @@ Module BedrockEvaluator (B : Heap) (ST : SepTheoryX.SepTheoryXType B).
       match s with
         | SymReg r => Some (Reg r)
         | SymImm e =>
-          match exprD funcs uvars vars e tvWord with
+          match exprD_repr e wIdx with
             | Some e => Some (Imm e)
             | None => None
           end
         | SymIndir r o =>
-          match exprD funcs uvars vars o tvWord with
+          match exprD_repr o wIdx with
             | Some o => Some (Indir r o)
             | None => None
           end
@@ -720,7 +724,7 @@ Module BedrockEvaluator (B : Heap) (ST : SepTheoryX.SepTheoryXType B).
                            | Some l => Some (RvLval l)
                            | None => None
                          end
-        | SymRvImm e => match exprD funcs uvars vars e tvWord with
+        | SymRvImm e => match exprD_repr e wIdx with
                           | Some l => Some (RvImm l)
                           | None => None
                         end
@@ -753,15 +757,29 @@ Module BedrockEvaluator (B : Heap) (ST : SepTheoryX.SepTheoryXType B).
 
     Definition regsD (r : regs) (sr : SymRegType) : Prop :=
       let '(sp, rp, rv) := sr in
-         exprD funcs uvars vars sp tvWord = Some (r Sp)
-      /\ exprD funcs uvars vars rp tvWord = Some (r Rp)
-      /\ exprD funcs uvars vars rv tvWord = Some (r Rv).
+         exprD_repr sp wIdx = Some (r Sp)
+      /\ exprD_repr rp wIdx = Some (r Rp)
+      /\ exprD_repr rv wIdx = Some (r Rv).
 
     Require Import PropX.
 
-    Definition stateD cs (stn : IL.settings) (s : state) (ss : SymState) : Prop :=
+    Definition sexprD_repr G (se : SepIL.ST.hprop (tvarD types wT) (tvarD types stT) G) : SepIL.hpropB G :=
+      let x := @cast_repr _ (fun t => 
+      SepIL.ST.hprop match t with
+                       | None => Empty_set
+                       | Some t => Impl t 
+                     end (tvarD types stT) G) deltaT types' wIdx se in
+      let x := @cast_repr _ (fun t => 
+      SepIL.ST.hprop W match t with
+                         | None => Empty_set
+                         | Some t => Impl t 
+                       end G) deltaT types' stIdx x in 
+      x.
+
+
+    Definition stateD cs (stn : settings) (s : state) (ss : SymState) : Prop :=
       PropX.interp cs ([| regsD (Regs s) (SymRegs ss) |] /\ 
-                       SepIL.SepFormula.sepFormula (SEP.sexprD funcs sfuncs uvars vars (SEP.sheapD (SymMem ss))) (stn, s))%PropX.
+                       SepIL.SepFormula.sepFormula (sexprD_repr (SEP.sexprD funcs sfuncs uvars vars (SEP.sheapD (SymMem ss)))) (stn, s))%PropX.
 
   End sym_denote.
 
@@ -796,17 +814,16 @@ Module BedrockEvaluator (B : Heap) (ST : SepTheoryX.SepTheoryXType B).
           forall rv,
           sym_evalRval r ss = Some rv ->
           exists rvD ,
-          exprD funcs uvars vars0 rv tvWord = Some rvD /\
+          exprD_repr uvars vars0 rv wIdx = Some rvD /\
           evalRvalue stn s rD = Some rvD.
         Proof.          
         Admitted.
-        Check sym_evalLval.
         Lemma sym_lvalue_sound : forall uvars vars0 l lD,
           sym_lvalueD uvars vars0 l = Some lD ->
           forall specs stn s ss, 
           stateD uvars vars0 specs stn s ss ->
           forall a aD ss',
-          exprD funcs uvars vars0 a tvWord = Some aD ->
+          exprD_repr uvars vars0 a wIdx = Some aD ->
           sym_evalLval l a ss = Some ss' ->
           exists s' , 
                evalLvalue stn s lD aD = Some s'
@@ -820,8 +837,11 @@ Module BedrockEvaluator (B : Heap) (ST : SepTheoryX.SepTheoryXType B).
             unfold stateD, regsD in *. PropXTac.propxFo.
               destruct (SymRegs ss). destruct p.
               destruct r; simpl in *; intuition.
-
-          
+            destruct ss; simpl in *. destruct SymRegs0. destruct p.
+            intuition.
+            Check SepIL.SepFormula.sepFormula.
+            rewrite SepIL.SepFormula.sepFormula_eq in *.
+            simpl in *.          
         Admitted.
         generalize dependent H2. case_eq (sym_evalRval s0 ss); try congruence.
         intros. eapply sym_rvalue_sound in H1; eauto. destruct H1. destruct H1.
@@ -831,6 +851,7 @@ Module BedrockEvaluator (B : Heap) (ST : SepTheoryX.SepTheoryXType B).
   Admitted.
 
 End BedrockEvaluator.
+*)
 
 
 (*
